some progress on list config equivalence

coq/pcc/temp2.v
@@ -8,7 +8,6 @@ Inductive configuration : Set :=
   | b  (_: nat)
   | b' (_: nat).
 
-
 Inductive trans : configuration -> configuration -> Prop :=
 (* [x] can go to anything *)
 | trans_xx    : trans x x
@@ -31,63 +30,190 @@ Inductive trans : configuration -> configuration -> Prop :=
 Hint Resolve trans_xx trans_xa trans_xb' trans_ab trans_a'x
   trans_a'a trans_a'b' trans_bx trans_ba trans_bb' trans_b'a' : transitions.
 
-
 Inductive execution : list configuration -> Prop :=
 | exec_nil : execution nil
-| exec_sing : forall c, execution (c :: nil)
+| exec_a : forall n, execution (a n :: nil)
+| exec_x : execution (x :: nil)
 | exec_trans : forall `(trans c c')
                  `(execution (e ++ (c :: nil))),
 	         execution (e ++ (c :: c' :: nil)).
 
-Definition test_conf_list := (x :: x :: (a 1) :: (b 1) :: x :: x :: (b' 5) :: nil).
-
+Definition test_conf_list := x :: x :: (a 1) :: (b 1) :: x :: x :: (b' 5) :: nil.
 
 Lemma rearrange (A: Set) : forall (a b c : A), a :: b :: c :: nil = (a :: nil) ++ (b :: c :: nil).
-  reflexivity.
-Qed.
+Proof. done. Qed.
 
 Lemma test_exec : execution test_conf_list.
 Proof.
-  unfold test_conf_list.
+  rewrite /test_conf_list.
   repeat (
     rewrite rearrange;
     repeat rewrite app_comm_cons;
     apply exec_trans;
     auto with transitions;
-    simpl).
-  
+    simpl).  
   apply exec_trans with (e := nil).
   apply trans_xx.
-
-  apply exec_sing.
+  apply exec_x.  
 Qed.
 
-
 Fixpoint a_updates (e : list configuration) : list nat :=
-match e with
-| nil => nil
-| a n :: e' => n :: a_updates e'
-| a' n :: e' => n :: a_updates e'
-| _ :: e' => a_updates e'
-end.
+  match e with
+    | nil => nil
+    | a n :: e' => n :: a_updates e'
+    | a' n :: e' => n :: a_updates e'
+    | _ :: e' => a_updates e'
+  end.
 
 Eval compute in a_updates test_conf_list.
 
 Fixpoint b_updates (e : list configuration) : list nat :=
 match e with
-| nil => nil
-| b n  :: e' => n :: b_updates e'
-| b' n :: e' => n :: b_updates e'
-| _  :: e' => b_updates e'
+  | nil => nil
+  | b n  :: e' => n :: b_updates e'
+  | b' n :: e' => n :: b_updates e'
+  | _  :: e' => b_updates e'
 end.
 
 Eval compute in b_updates test_conf_list.
 
 Lemma test_conf_exists : exists e', (execution e') /\ b_updates test_conf_list = a_updates e'.
+Proof. 
+ exists (x :: x :: a 1 :: b 1 :: x :: x :: b' 5 :: a' 5 :: nil).
+ split.
+ - repeat (
+    rewrite rearrange;
+    repeat rewrite app_comm_cons;
+    apply exec_trans;
+    auto with transitions;
+    simpl).  
+   apply exec_trans with (e := nil).
+   * by apply trans_xx.
+   * by apply exec_x.
+ - by done.
+Qed.
+
+Lemma rev_case : forall (e : list configuration), e = nil \/ (exists e', exists c, e = e' ++ (c :: nil)).
 Proof.
+ elim/rev_ind => [|c e].
+ - by left.
+ - move => H.
+   elim: H => H.
+   * right.
+     rewrite H.
+     exists nil.
+     exists c.
+     done.
+   * right.
+     elim: H => e' H.
+     elim: H => c' H.
+     rewrite H {H}.
+     exists (e' ++ c' :: nil).
+     exists c.
+     by rewrite app_ass -app_comm_cons.
+Qed.
+
+Lemma b_updates_ignores_x : forall `(execution e), b_updates (e ++ x :: nil) = b_updates e.
 Admitted.
- 
+
+Lemma b_updates_ignores_an : forall `(execution e) (n : nat), b_updates (e ++ a n :: nil) = b_updates e.
+Admitted.
+
 Lemma exists_exec_with_eq_bs :
   forall `(execution e), exists e', (execution e') /\ b_updates e = a_updates e'.
 Proof.
+ elim/rev_ind => [H|c e].
+ - exists nil.
+   split.
+   * by apply exec_nil.
+   * by done.
+ - pose proof rev_case e.
+   elim: H => H.
+   * rewrite H {H}.
+     case:c => [H0 H1|n H0 H1|n H0 H1|n H0 H1|n H0 H1].
+     + by exists (x :: nil); split; [ apply exec_x | done].
+     + by exists nil; split; [ apply exec_nil | done ].
+     + by exists nil; split; [ apply exec_nil | done ].
+     + exists (a n :: nil); split.
+       - inversion H1.
+         by apply exec_a.
+       - by done.
+     + exists (a n :: nil); split.
+       - inversion H1.
+         by apply exec_a.
+       - by done.
+   * elim: H => e' H.
+     elim: H => c' H.
+     rewrite H {H}.
+     move => IH H.
+     have H0: (e' ++ c' :: nil) ++ c :: nil = e' ++ (c' :: c :: nil) by rewrite app_ass -app_comm_cons.
+     rewrite H0 in H.
+     rewrite H0 {H0}.
+     inversion H.
+     + by exists nil; split; [ apply exec_nil | done ].
+     + by exists nil; split; [ apply exec_nil | done ].
+     + by exists (x :: nil); split; [ apply exec_x | done ].
+     + have H2: (e0 ++ (c0 :: c'0 :: nil) = (e0 ++ c0 :: nil) ++ c'0 :: nil) by rewrite -ass_app -app_comm_cons.
+       rewrite H2 {H2} in H1.
+       have H2: (e' ++ (c' :: c :: nil) = (e' ++ c' :: nil) ++ c :: nil) by rewrite -ass_app -app_comm_cons.
+       rewrite H2 {H2} in H1.
+       apply app_inj_tail in H1.
+       elim: H1 => H1 H2.
+       apply app_inj_tail in H1.
+       elim: H1 => H1 H3.
+       rewrite H2 in trans0.
+       rewrite H2 {H2 c'0}.
+       rewrite H1 in execution0.
+       rewrite H1 {H1 e0}.
+       rewrite H3 in execution0.
+       rewrite H3 in trans0.
+       rewrite H3 {H3 c0}.
+       have H0: execution (e' ++ c' :: nil) by apply execution0.
+       apply IH in H0.
+       elim: H0 => e0 H0 {IH}.
+       elim: H0 => H0 H1.
+       move: H H1 trans0.       
+       case c => [H H1 trans0|n H H1 trans0|||].
+       - exists e0; split; first done.
+         have H2: e' ++ c' :: x :: nil = (e' ++ c' :: nil) ++ x :: nil by rewrite -ass_app -app_comm_cons.
+         rewrite H2 {H2}.         
+         by rewrite b_updates_ignores_x. 
+       - exists e0; split; first done.
+         rewrite -H1 {H1}.
+         have H2: e' ++ c' :: a n :: nil = (e' ++ c' :: nil) ++ a n :: nil by rewrite -ass_app -app_comm_cons.
+         rewrite H2 {H2}.
+         
+
+
+inversion trans0.
+         subst.
+         exists e0; split; first done.
+         rewrite -H1 {H1}.
+         Focus 2.
+       - 
+       
+       rewrite 
+
+       rew
+       rewrite -ass_app.
+       rewrite -app_comm_cons.
+
+apply app_inj_tail in H1.
+     + have H2: e' = e'.
+       
+
+move => IH.
+     
+     rewrite H {H} => H.
+     
+     
+   
+   
+       exists (c :: nil).
+   split; first by rewrite /= in H1; apply H1.
+   
+
+case H: e => [|c' e0].
+   * 
+
 Admitted.
